## Factored sum of powers polynomials

Using the above script, I computed the [coefficients of $f_p$ from power $0$ to power $99$](sumpow.html). Below are $f_p$ from power $1$ to power $10$ as well as their factored form:

$f_1(n)={\sum_{k=1}^{n}k^{1}=\frac{1}{2}n^{2}+\frac{1}{2}n=\frac{1}{2}n\left(n+1\right)}$

$f_2(n)={\sum_{k=1}^{n}k^{2}=\frac{1}{3}n^{3}+\frac{1}{2}n^{2}+\frac{1}{6}n=\frac{1}{6}n\left(n+1\right)\left(2n+1\right)}$

$f_3(n)={\sum_{k=1}^{n}k^{3}=\frac{1}{4}n^{4}+\frac{1}{2}n^{3}+\frac{1}{4}n^{2}=\frac{1}{4}n^{2}\left(n+1\right)^{2}}$

$f_4(n)={\sum_{k=1}^{n}k^{4}=\frac{1}{5}n^{5}+\frac{1}{2}n^{4}+\frac{1}{3}n^{3}-\frac{1}{30}n=\frac{1}{30}n\left(n+1\right)\left(2n+1\right)\left(3n^{2}+3n-1\right)}$

$f_5(n)={\sum_{k=1}^{n}k^{5}=\frac{1}{6}n^{6}+\frac{1}{2}n^{5}+\frac{5}{12}n^{4}-\frac{1}{12}n^{2}=\frac{1}{12}n^{2}\left(n+1\right)^{2}\left(2n^{2}+2n-1\right)}$

$f_6(n)={\sum_{k=1}^{n}k^{6}=\frac{1}{7}n^{7}+\frac{1}{2}n^{6}+\frac{1}{2}n^{5}-\frac{1}{6}n^{3}+\frac{1}{42}n=\frac{1}{42}n\left(n+1\right)\left(2n+1\right)\left(3n^{4}+6n^{3}-3n+1\right)}$

$f_7(n)={\sum_{k=1}^{n}k^{7}=\frac{1}{8}n^{8}+\frac{1}{2}n^{7}+\frac{7}{12}n^{6}-\frac{7}{24}n^{4}+\frac{1}{12}n^{2}=\frac{1}{24}n^{2}\left(n+1\right)^{2}\left(3n^{4}+6n^{3}-n^{2}-4n+2\right)}$

$f_8(n)={\sum_{k=1}^{n}k^{8}=\frac{1}{9}n^{9}+\frac{1}{2}n^{8}+\frac{2}{3}n^{7}-\frac{7}{15}n^{5}+\frac{2}{9}n^{3}-\frac{1}{30}n=\frac{1}{90}n\left(n+1\right)\left(2n+1\right)\left(5n^{6}+15n^{5}+5n^{4}-15n^{3}-n^{2}+9n-3\right)}$

$f_9(n)={\sum_{k=1}^{n}k^{9}=\frac{1}{10}n^{10}+\frac{1}{2}n^{9}+\frac{3}{4}n^{8}-\frac{7}{10}n^{6}+\frac{1}{2}n^{4}-\frac{3}{20}n^{2}=\frac{1}{20}n^{2}\left(n+1\right)^{2}\left(n^{2}+n-1\right)\left(2n^{4}+4n^{3}-n^{2}-3n+3\right)}$

$f_{10}(n)={\sum_{k=1}^{n}k^{10}=\frac{1}{11}n^{11}+\frac{1}{2}n^{10}+\frac{5}{6}n^{9}-n^{7}+n^{5}-\frac{1}{2}n^{3}+\frac{5}{66}n\\=\frac{1}{66}n\left(n+1\right)\left(2n+1\right)\left(n^{2}+n-1\right)\left(3n^{6}+9n^{5}+2n^{4}-11n^{3}+3n^{2}+10n-5\right)}$

One should notice some patterns in the polynomials:

- When terms are written in decreasing power, the polynomial $f_p$ always begins with $\dfrac{1}{p+1}n^{p+1}+\dfrac{1}{2}n^p$;

- For $p\ge 2$, $f_p$ always contain factor $\dfrac{1}{6}n(n+1)(2n+1)$ when $p$ is even and factor $\dfrac{1}{4}n^2(n+1)^2$ when $p$ is odd.

Two years ago, when I first generated these equations, I could explain:

- $f_p(n)$ contains factor $n$ because $f_p(0)$ is always $0$, $n=0$ is a root of $f_p$, so $f_p$ contains factor $n-0=n$;

- Since $f_p(n)=n^p+f_p(n-1)$, $f_p(n-1)=f_p(n)-n^p$, $f_p(-1)=f_p(0)-0^p=f_p(0)=0$, $n=-1$ is a root of $f_p$, so $f_p$ also contains factor $n+1$;

- $\dfrac{1}{4}n^2(n+1)^2$ is integer because one of $n$ and $n+1$ must be even and so $n^2(n+1)^2$ is divisible by 4;

- One of $n$ and $n+1$ must be even so $n(n+1)(2n+1)$ contains factor 2; When $n\equiv 1 (\mod 3)$, $2n+1$ is divisible by 3; when $n\equiv 2 (\mod 3)$, $n+1$ is divisible by 3; otherwise $n$ is divisible by 3, so $n(n+1)(2n+1)$ also contains factor 3. $n(n+1)(2n+1)$ is divisible by both $2$ and $3$ so $\dfrac{1}{6}n(n+1)(2n+1)$ is integer.

I couldn't explain why $f_p$ always begin with $\dfrac{1}{p+1}n^{p+1}+\dfrac{1}{2}n^p$ and didn't know why $n(n+1)(2n+1)$ and $n^2(n+1)^2$ appear as factors of $f_p$.

